examples/dsls/mini_steel/Pulse.Soundness.Common.fst
@@ -295,10 +295,10 @@ let sub_stt_type u =
 let stt_env = 
   f:RT.fstar_top_env {
     RT.lookup_fvar f RT.bool_fv == Some (RT.tm_type RT.u_zero) /\
-    RT.lookup_fvar f vprop_fv == Some (RT.tm_type (elab_universe (U_succ (U_succ U_zero)))) /\ True
-    //(forall (u1 u2:R.universe). RT.lookup_fvar_uinst f bind_fv [u1; u2] == Some (bind_type u1 u2)) /\
-    //(forall (u:R.universe). RT.lookup_fvar_uinst f frame_fv [u] == Some (frame_type u)) /\
-    //(forall (u:R.universe). RT.lookup_fvar_uinst f subsumption_fv [u] == Some (sub_stt_type u))        
+    RT.lookup_fvar f vprop_fv == Some (RT.tm_type (elab_universe (U_succ (U_succ U_zero)))) /\
+    (forall (u1 u2:R.universe). RT.lookup_fvar_uinst f bind_fv [u1; u2] == Some (bind_type u1 u2)) /\
+    (forall (u:R.universe). RT.lookup_fvar_uinst f frame_fv [u] == Some (frame_type u)) /\
+    (forall (u:R.universe). RT.lookup_fvar_uinst f subsumption_fv [u] == Some (sub_stt_type u))        
   }
 
 let check_top_level_environment (f:RT.fstar_top_env)
