examples/dsls/mini_steel/Pulse.Soundness.fst
@@ -14,6 +14,7 @@ module Frame = Pulse.Soundness.Frame
 module STEquiv = Pulse.Soundness.STEquiv
 module Return = Pulse.Soundness.Return
 
+
 #push-options "--query_stats --fuel 2 --ifuel 2 --z3rlimit_factor 10"
 let rec soundness (f:stt_env)
                   (g:env)
@@ -40,6 +41,28 @@ let rec soundness (f:stt_env)
         mk_t_abs f g ppname r_t_typing r_body_typing
     in
     match d with
+    | T_Tot _ _ _ d -> d
+
+    | T_Abs _ ppname x q ty u body c hint _ t_typing body_typing ->
+      mk_t_abs q ppname t_typing body_typing    
+
+
+    | T_STApp _ head ppname formal q res arg head_typing arg_typing ->
+      let E arg_typing = arg_typing in
+      let r_head = elab_src_typing head_typing in
+      let r_arg = elab_pure arg in
+      elab_pure_equiv arg_typing;
+      let r_head_typing
+        : RT.typing _ r_head (elab_pure (Tm_Arrow {binder_ty=formal;binder_ppname=ppname} q res))
+        = soundness _ _ _ _ head_typing
+      in
+      let r_arg_typing = soundness _ _ _ _ arg_typing in
+      elab_comp_open_commute res arg;
+      RT.T_App _ _ _ (binder_of_t_q_s (elab_pure formal) (elab_qual q) ppname)
+                     (elab_pure_comp res)
+                     r_head_typing
+                     r_arg_typing
+
     | T_Bind _ e1 e2 c1 c2 x c e1_typing t_typing e2_typing bc ->
       if C_ST? c1 && C_ST? c2 then
       let r1_typing
@@ -57,53 +80,27 @@ let rec soundness (f:stt_env)
                             (tot_typing_soundness t2_typing)
                             (mk_t_abs_tot _ _ _ t2_typing post2_typing)
       else admit ()
+    | T_Frame _ e c frame frame_typing e_typing ->
+      if C_ST? c then
+      let r_e_typing = soundness _ _ _ _ e_typing in
+      assume (ln_c c);
+      Frame.elab_frame_typing f g _ _ frame frame_typing r_e_typing
+      else admit ()
 
-    | _ -> admit ()
+    | T_Equiv _ e c c' e_typing equiv ->
+      if C_ST? c && C_ST? c' then begin
+      assume (ln_c c /\ ln_c c');
+      let r_e_typing = soundness _ _ _ _ e_typing in 
+      STEquiv.st_equiv_soundness _ _ _ _ equiv _ r_e_typing
+      end
+      else admit ()
 
-    // | T_Tot _ _ _ d -> d
+    | T_Return _ e t u e_typing t_typing ->
+      Return.elab_return_typing t_typing e_typing
 
-    // | T_Abs _ ppname x q ty u body c hint _ t_typing body_typing ->
-    //   mk_t_abs q ppname t_typing body_typing    
-
-
-    // | T_STApp _ head ppname formal q res arg head_typing arg_typing ->
-    //   let E arg_typing = arg_typing in
-    //   let r_head = elab_src_typing head_typing in
-    //   let r_arg = elab_pure arg in
-    //   elab_pure_equiv arg_typing;
-    //   let r_head_typing
-    //     : RT.typing _ r_head (elab_pure (Tm_Arrow {binder_ty=formal;binder_ppname=ppname} q res))
-    //     = soundness _ _ _ _ head_typing
-    //   in
-    //   let r_arg_typing = soundness _ _ _ _ arg_typing in
-    //   elab_comp_open_commute res arg;
-    //   RT.T_App _ _ _ (binder_of_t_q_s (elab_pure formal) (elab_qual q) ppname)
-    //                  (elab_pure_comp res)
-    //                  r_head_typing
-    //                  r_arg_typing
-
-
-    // | T_Frame _ e c frame frame_typing e_typing ->
-    //   if C_ST? c then
-    //   let r_e_typing = soundness _ _ _ _ e_typing in
-    //   assume (ln_c c);
-    //   Frame.elab_frame_typing f g _ _ frame frame_typing r_e_typing
-    //   else admit ()
-
-    // | T_Equiv _ e c c' e_typing equiv ->
-    //   if C_ST? c && C_ST? c' then begin
-    //   assume (ln_c c /\ ln_c c');
-    //   let r_e_typing = soundness _ _ _ _ e_typing in 
-    //   STEquiv.st_equiv_soundness _ _ _ _ equiv _ r_e_typing
-    //   end
-    //   else admit ()
-
-    // | T_Return _ e t u e_typing t_typing ->
-    //   Return.elab_return_typing t_typing e_typing
-
-    // | T_ReturnNoEq _ e t u e_typing t_typing ->
-    //   let e_typing = soundness _ _ _ _ e_typing in
-    //   Return.elab_return_noeq_typing t_typing e_typing
+    | T_ReturnNoEq _ e t u e_typing t_typing ->
+      let e_typing = soundness _ _ _ _ e_typing in
+      Return.elab_return_noeq_typing t_typing e_typing
       
     // | T_If  -> admit()
 
